prove AC1, and bug fixes to protocol

exercise03.dfy
@@ -11,50 +11,94 @@ module TwoPCInvariantProof {
   import opened DistributedSystem
   import opened Obligations
 
-/*{*/
-/*}*/
-  // This is a conjunct of the inductive invariant, indicating that the messages carrying
-  // decisions should reflect the votes of the participants as relayed to the coordinator
-  predicate DecisionMsgsAgreeWithDecision(c: Constants, v: Variables)
+
+
+  // // DecideMsgs should reflect the decision of the leader
+  // // Tony: Boilerplate
+  // predicate DecisionMsgsAgreeWithTally(c: Constants, v: Variables)
+  //   requires v.WF(c)
+  // {
+  //   forall msg | msg in v.network.sentMsgs && msg.DecideMsg? 
+  //   :: GetCoordinator(c, v).decision.Some? && msg.d == GetCoordinator(c, v).decision.value
+  // }
+
+  // DecideMsgs should reflect the decision of the leader
+  // Tony: Boilerplate
+  predicate DecisionMsgsAgreeWithLeader(c: Constants, v: Variables)
     requires v.WF(c)
   {
-/*{*/
-    true // Replace me
-/*}*/
+    forall msg | msg in v.network.sentMsgs && msg.DecideMsg? 
+    :: GetCoordinator(c, v).decision.Some? && msg.d == GetCoordinator(c, v).decision.value
   }
+
+  // If a participant has decided, then there must be a corresponding DecideMsg
+  // Tony: Boilerplate
+  predicate ParticipantsDecisionImpliesDecideMsg(c: Constants, v: Variables) 
+    requires v.WF(c)
+  {
+    var n := |v.hosts|;
+    forall i | 0 <= i < n && HostHasDecided(v.hosts[i]) :: 
+      && (HostDecidedCommit(v.hosts[i]) ==> DecideMsg(Commit) in v.network.sentMsgs)
+      && (HostDecidedAbort(v.hosts[i]) ==> DecideMsg(Abort) in v.network.sentMsgs)
+  }
+
+  // There can only be one DecideMsg in the network
+  // I think this is implied by from DecisionMsgsAgreeWithLeaderDecision
+  // predicate OnlyOneDecisionMsg(c: Constants, v: Variables)
+  //   requires v.WF(c)
+  // {
+  //   var sentMsgs := v.network.sentMsgs;
+  //   forall m1, m2 | m1 in sentMsgs && m1.DecideMsg? && m2 in sentMsgs && m2.DecideMsg? 
+  //   :: m1 == m2
+  // }
+
+  // If a DecideMsg(Commit) message is in the network, every host that decides must 
+  // decide Commit, and likewise for Abort.
+  // I think this is implied by OnlyOneDecisionMsg
+  // predicate HostsAgreeWithDecisionMsg(c: Constants, v: Variables)
+  //   requires v.WF(c)
+  // {
+  //   var n := |v.hosts|;
+  //   && (DecideMsg(Commit) in v.network.sentMsgs ==> 
+  //     forall i | 0 <= i < n && HostHasDecided(v.hosts[i]) :: HostDecidedCommit(v.hosts[i])
+  //   )
+  //   && (DecideMsg(Abort) in v.network.sentMsgs ==> 
+  //     forall i | 0 <= i < n && HostHasDecided(v.hosts[i]) :: HostDecidedAbort(v.hosts[i])
+  //   )
+  // }
+
+
 
   predicate Inv(c: Constants, v: Variables)
   {
     && v.WF(c)
-/*{*/
-/*}*/
-    // We give you the blueprint for one invariant to get you started...
-    && DecisionMsgsAgreeWithDecision(c, v)
-    // ...but you'll need more.
+    && DecisionMsgsAgreeWithLeader(c, v)
+    && ParticipantsDecisionImpliesDecideMsg(c, v)
     && Safety(c, v)
   }
 
   lemma InitImpliesInv(c: Constants, v: Variables)
     requires Init(c, v)
     ensures Inv(c, v)
-  {
-/*{*/
-/*}*/
-  }
+  {}
 
+
+  /*
+    - DecisionMsgsAgreeWithLeader(c, v) and ParticipantsDecisionImpliesDecideMsg(c, v) implies AC1
+      AC1 + these two invariants are inductive.
+  */
   lemma InvInductive(c: Constants, v: Variables, v': Variables)
     requires Inv(c, v)
     requires Next(c, v, v')
     ensures Inv(c, v')
   {
-/*{*/
-/*}*/
+    assert SafetyAC1(c, v');
+    assert Inv(c, v');
   }
 
   lemma InvImpliesSafety(c: Constants, v: Variables)
     requires Inv(c, v)
     ensures Safety(c, v)
-  { // Trivial, as usual, since safety is a conjunct in Inv.
-  }
+  {}
 }
 
