exercise02.dfy
@@ -28,40 +28,6 @@ module Obligations {
 
 /*{*/
 /*}*/
-
-  predicate HostHasDecided(h: Host.Variables) {
-    match h
-      case CoordinatorVariables(c) => c.decision.Some?
-      case ParticipantVariables(p) => p.decision.Some?
-  }
-
-  predicate HostDecidedCommit(h: Host.Variables) {
-    match h
-      case CoordinatorVariables(c) => c.decision == Some(Commit)
-      case ParticipantVariables(p) => p.decision == Some(Commit)
-  }
-
-  predicate HostDecidedAbort(h: Host.Variables) {
-    match h
-      case CoordinatorVariables(c) => c.decision == Some(Abort)
-      case ParticipantVariables(p) => p.decision == Some(Abort)
-  }
-
-  predicate HostsReachSameDecision(h1: Host.Variables, h2: Host.Variables) 
-    requires HostHasDecided(h1)
-    requires HostHasDecided(h2)
-  {
-    (HostDecidedCommit(h1) && HostDecidedCommit(h2)) || (HostDecidedAbort(h1) && HostDecidedAbort(h2))
-  }
-
-  predicate AllPreferYes(c: Constants, v: Variables) 
-    requires v.WF(c)
-  {
-    var n := |c.hosts|;
-    forall j | 0 <= j < n-1 :: c.hosts[j].participant.preference == Yes
-  }
-
-
   // AC-1: All processes that reach a decision reach the same one.
   predicate SafetyAC1(c: Constants, v: Variables)
     requires v.WF(c)
@@ -106,7 +72,59 @@ module Obligations {
     requires v.WF(c)
   {
     && SafetyAC1(c, v)
-    && SafetyAC3(c, v)
-    && SafetyAC4(c, v)
+    // && SafetyAC3(c, v)
+    // && SafetyAC4(c, v)
+  }
+
+
+
+
+  /***************************************************************************************
+  *                                      Utils                                           *
+  ***************************************************************************************/
+
+  function GetCoordinator(c: Constants, v: Variables) : CoordinatorHost.Variables
+    requires v.WF(c)
+  {
+    Last(v.hosts).coordinator
+  }
+
+  function GetParticipant(c: Constants, v: Variables, i: int) : ParticipantHost.Variables
+    requires v.WF(c)
+    requires 0 <= i < |v.hosts|-1
+  {
+    v.hosts[i].participant
+  }
+
+  predicate HostHasDecided(h: Host.Variables) {
+    match h
+      case CoordinatorVariables(c) => c.decision.Some?
+      case ParticipantVariables(p) => p.decision.Some?
+  }
+
+  predicate HostDecidedCommit(h: Host.Variables) {
+    match h
+      case CoordinatorVariables(c) => c.decision == Some(Commit)
+      case ParticipantVariables(p) => p.decision == Some(Commit)
+  }
+
+  predicate HostDecidedAbort(h: Host.Variables) {
+    match h
+      case CoordinatorVariables(c) => c.decision == Some(Abort)
+      case ParticipantVariables(p) => p.decision == Some(Abort)
+  }
+
+  predicate HostsReachSameDecision(h1: Host.Variables, h2: Host.Variables) 
+    requires HostHasDecided(h1)
+    requires HostHasDecided(h2)
+  {
+    (HostDecidedCommit(h1) && HostDecidedCommit(h2)) || (HostDecidedAbort(h1) && HostDecidedAbort(h2))
+  }
+
+  predicate AllPreferYes(c: Constants, v: Variables) 
+    requires v.WF(c)
+  {
+    var n := |c.hosts|;
+    forall j | 0 <= j < n-1 :: c.hosts[j].participant.preference == Yes
   }
 }
